Foundation/Modal/Kripke/Hilbert/S4Dot3.lean
@@ -28,44 +28,8 @@ instance Kripke.sound : Sound (Hilbert.S4Dot3) ReflexiveTransitiveConnectedFrame
 instance Kripke.consistent : Entailment.Consistent (Hilbert.S4Dot3) :=
   Kripke.Hilbert.consistent_of_FrameClass Kripke.ReflexiveTransitiveConnectedFrameClass
 
-
-open
-  Kripke
-  MaximalConsistentSet
-in
-instance Kripke.canonical : Canonical (Hilbert.S4Dot3) ReflexiveTransitiveConnectedFrameClass := by
-  have hS4 := canonicalFrame.multigeachean_of_provable_geach (G := {⟨0, 0, 1, 0⟩, ⟨0, 2, 1, 0⟩}) (𝓢 := Hilbert.S4Dot3) (by simp);
-  constructor;
-  refine ⟨?_, ?_, ?_⟩;
-  . simpa [reflexive_def] using @hS4 (⟨0, 0, 1, 0⟩) $ by tauto;
-  . simpa [transitive_def] using @hS4 ⟨0, 2, 1, 0⟩ $ by tauto;
-  . intro X Y Z ⟨hXY, hXZ⟩;
-    by_contra hC;
-    push_neg at hC;
-    have ⟨hnYZ, hnZY⟩ := hC; clear hC;
-    simp only [Set.not_subset] at hnYZ hnZY;
-    obtain ⟨φ, hpY, hpZ⟩ := hnYZ; replace hpY : □φ ∈ Y := hpY;
-    obtain ⟨ψ, hqZ, hqY⟩ := hnZY; replace hqZ : □ψ ∈ Z := hqZ;
-    have hpqX : □(□φ ➝ ψ) ∉ X := by
-      apply iff_mem_box.not.mpr;
-      push_neg;
-      use Y;
-      constructor;
-      . assumption;
-      . apply iff_mem_imp.not.mpr;
-        aesop;
-    have hqpX : □(□ψ ➝ φ) ∉ X := by
-      apply iff_mem_box.not.mpr; push_neg;
-      use Z;
-      constructor;
-      . assumption;
-      . apply iff_mem_imp.not.mpr;
-        aesop;
-    have : (□(□φ ➝ ψ) ⋎ □(□ψ ➝ φ)) ∉ X := by apply iff_mem_or.not.mpr; push_neg; exact ⟨hpqX, hqpX⟩;
-    have : □(□φ ➝ ψ) ⋎ □(□ψ ➝ φ) ∈ X := by
-      apply membership_iff.mpr;
-      exact Entailment.axiomDot3!;
-    contradiction;
+instance Kripke.canonical : Canonical (Hilbert.S4Dot3) ReflexiveTransitiveConnectedFrameClass :=
+  ⟨⟨Canonical.reflexive, Canonical.transitive, Canonical.connected⟩⟩
 
 instance Kripke.complete : Complete (Hilbert.S4Dot3) ReflexiveTransitiveConnectedFrameClass := inferInstance
 
